whole_prog_thm for yes (string version)
Proof largely by copypasting from cyes

examples/cost/yesProgScript.sml
@@ -92,6 +92,395 @@ val yes2 =
   in (rhs o concl o EVAL) ``^whole_prog ++ ^prog``
   end
 
+(* A small IO model *)
+open cfDivTheory;
+
+val names_def = Define `names = ["put_char"]`;
+
+val put_char_event_def = Define `
+  put_char_event c = IO_event "put_char" [n2w (ORD c)] []`;
+
+val put_str_event_def = Define `
+  put_str_event cs = IO_event "put_char" (MAP (n2w o ORD) (explode cs)) []`;
+
+val update_def = Define `
+  (update "put_char" cs l s = SOME (FFIreturn l s))`
+
+val State_def = Define `
+  State = Stream [||]`
+
+val SIO_def = Define `
+  SIO events =
+    one (FFI_part (State) update names events)`
+
+val st = ml_translatorLib.get_ml_prog_state();
+
+Theorem put_line_spec:
+  !s sv events.
+  limited_parts names p /\ STRING_TYPE s sv ==>
+  app (p:'ffi ffi_proj) ^(fetch_v "put_line" st) [sv]
+    (SIO events)
+    (POSTv v. &UNIT_TYPE () v *
+              SIO (SNOC (put_str_event (s ^ strlit "\n")) events))
+Proof
+  xcf "put_line" st
+  \\ xlet `POSTv v. &STRING_TYPE (strcat s (strlit "\n")) v * SIO events`
+  THEN1 (xapp \\ xsimpl \\ goal_assum drule \\ rw[])
+  \\ xlet `POSTv v. &WORD8 0w v * SIO events` THEN1 (xapp \\ xsimpl)
+  \\ xlet `POSTv v. W8ARRAY v [] * SIO events` THEN1 (xapp \\ xsimpl \\ goal_assum drule)
+  \\ rename1 `W8ARRAY av`
+  \\ xlet
+    `POSTv v. &UNIT_TYPE () v * W8ARRAY av [] *
+              SIO (SNOC (put_str_event (s ^ strlit "\n")) events)`
+  THEN1 (
+    xffi \\ xsimpl \\ fs [SIO_def]
+    \\ MAP_EVERY qexists_tac
+      [`MAP (n2w o ORD) (explode(s ^ strlit "\n"))`, `emp`, `State`, `update`, `names`, `events`]
+    \\ fs [update_def, put_str_event_def, names_def, SNOC_APPEND,
+           implode_def, STRING_TYPE_def, State_def,strcat_thm,concat_thm,
+           MAP_MAP_o,CHR_w2n_n2w_ORD]
+    \\ xsimpl)
+  \\ xcon \\ xsimpl
+QED
+
+(* TODO: Move REPLICATE_LIST and lemmas to an appropriate theory;
+         this is copypasted from divScript *)
+
+val REPLICATE_LIST_def = Define `
+  (!l. REPLICATE_LIST l 0 = []) /\
+  (!l n. REPLICATE_LIST l (SUC n) = REPLICATE_LIST l n ++ l)`
+
+Theorem REPLICATE_LIST_SNOC:
+  !x n. SNOC x (REPLICATE_LIST [x] n) = REPLICATE_LIST [x] (SUC n)
+Proof
+  rw [REPLICATE_LIST_def]
+QED
+
+Theorem REPLICATE_LIST_APPEND:
+  !l n. REPLICATE_LIST l n ++ l = REPLICATE_LIST l (SUC n)
+Proof
+  rw [REPLICATE_LIST_def]
+QED
+
+Theorem REPLICATE_LIST_APPEND_SYM:
+  !l n. REPLICATE_LIST l n ++ l = l ++ REPLICATE_LIST l n
+Proof
+  strip_tac \\ Induct_on `n` \\ fs [REPLICATE_LIST_def]
+QED
+
+Theorem REPLICATE_LIST_LENGTH:
+  !l n. LENGTH (REPLICATE_LIST l n) = LENGTH l * n
+Proof
+  Induct_on `n` THEN1 (EVAL_TAC \\ fs [])
+  \\ rw [REPLICATE_LIST_def, MULT_CLAUSES]
+QED
+
+Theorem LPREFIX_REPLICATE_LIST_LREPEAT:
+  !l n. LPREFIX (fromList (REPLICATE_LIST l n)) (LREPEAT l)
+Proof
+  strip_tac \\ Induct_on `n`
+  \\ fs [REPLICATE_LIST_def, REPLICATE_LIST_APPEND_SYM, GSYM LAPPEND_fromList]
+  \\ rw [Once LREPEAT_thm] \\ fs [LPREFIX_APPEND]
+  \\ qexists_tac `ll` \\ fs [LAPPEND_ASSOC]
+QED
+
+Theorem LTAKE_EQ_MULT:
+  !ll1 ll2 m.
+    0 < m /\ ~LFINITE ll1 /\
+    (!n. LTAKE (m * n) ll1 = LTAKE (m * n) ll2) ==>
+    (!n. LTAKE n ll1 = LTAKE n ll2)
+Proof
+  rw []
+  \\ first_x_assum (qspec_then `n` mp_tac) \\ strip_tac
+  \\ drule NOT_LFINITE_TAKE
+  \\ disch_then (qspec_then `m * n` mp_tac) \\ strip_tac \\ fs []
+  \\ rename1 `SOME l`
+  \\ `n <= m * n` by fs []
+  \\ `LTAKE n ll1 = SOME (TAKE n l)` by (
+    irule LTAKE_TAKE_LESS \\ qexists_tac `m * n` \\ fs [])
+  \\ `LTAKE n ll2 = SOME (TAKE n l)` by (
+    irule LTAKE_TAKE_LESS \\ qexists_tac `m * n` \\ fs [])
+  \\ fs []
+QED
+
+Theorem LTAKE_LAPPEND_fromList:
+  !ll l n.
+    LTAKE (n + LENGTH l) (LAPPEND (fromList l) ll) =
+      OPTION_MAP (APPEND l) (LTAKE n ll)
+Proof
+  rw [] \\ Cases_on `LTAKE n ll` \\ fs []
+  THEN1 (
+    `LFINITE ll` by (fs [LFINITE] \\ instantiate)
+    \\ drule LFINITE_HAS_LENGTH \\ strip_tac \\ rename1 `SOME m`
+    \\ irule LTAKE_LLENGTH_NONE
+    \\ qexists_tac `m + LENGTH l` \\ rw []
+    THEN1 (
+      drule LTAKE_LLENGTH_SOME \\ strip_tac
+      \\ Cases_on `n ≤ m` \\ fs []
+      \\ drule (GEN_ALL LTAKE_TAKE_LESS)
+      \\ disch_then drule \\ fs [])
+    \\ fs [LLENGTH_APPEND, LFINITE_fromList])
+  \\ Induct_on `l` \\ rw []
+  \\ fs [LTAKE_CONS_EQ_SOME]
+  \\ instantiate
+QED
+
+Theorem REPLICATE_LIST_LREPEAT:
+  !l ll.
+    l <> [] /\ (!n. LPREFIX (fromList (REPLICATE_LIST l n)) ll) ==>
+    (ll = LREPEAT l)
+Proof
+  rw [LTAKE_EQ]
+  \\ Cases_on `toList ll`
+  THEN1 (
+    irule LTAKE_EQ_MULT
+    \\ `~LFINITE ll` by fs [LFINITE_toList_SOME] \\ fs []
+    \\ qexists_tac `LENGTH l`
+    \\ `0 < LENGTH l` by (Cases_on `l` \\ fs []) \\ rw []
+    \\ rpt (pop_assum mp_tac) \\ qid_spec_tac `ll`
+    \\ Induct_on `n` \\ rw []
+    \\ `?ll1. ll = LAPPEND (fromList l) ll1` by (
+      first_x_assum (qspec_then `1` mp_tac) \\ strip_tac
+      \\ fs [LPREFIX_APPEND, EVAL ``REPLICATE_LIST l 1``]
+      \\ rename1 `LAPPEND _ ll1`
+      \\ qexists_tac `ll1` \\ fs [])
+    \\ `~LFINITE ll1` by fs [LFINITE_APPEND, LFINITE_fromList]
+    \\ `toList ll1 = NONE` by fs [LFINITE_toList_SOME]
+    \\ `!n. LPREFIX (fromList (REPLICATE_LIST l n)) ll1` by (
+      strip_tac \\ rename1 `REPLICATE_LIST _ n1`
+      \\ first_x_assum (qspec_then `SUC n1` mp_tac) \\ strip_tac
+      \\ fs [LPREFIX_fromList] \\ rfs []
+      \\ fs [REPLICATE_LIST_LENGTH, MULT_CLAUSES]
+      \\ qspecl_then [`ll1`, `l`, `n1 * LENGTH l`] mp_tac
+                     LTAKE_LAPPEND_fromList \\ strip_tac
+      \\ fs [REPLICATE_LIST_def, REPLICATE_LIST_APPEND_SYM])
+    \\ first_x_assum (qspec_then `ll1` drule)
+    \\ rpt (disch_then drule) \\ strip_tac \\ rveq
+    \\ `LENGTH l * SUC n = LENGTH l * n + LENGTH l` by fs [MULT_CLAUSES]
+    \\ qspecl_then [`ll1`, `l`, `LENGTH l * n`] mp_tac
+                   LTAKE_LAPPEND_fromList \\ strip_tac
+    \\ rw [Once LREPEAT_thm]
+    \\ qspecl_then [`LREPEAT l`, `l`, `LENGTH l * n`] mp_tac
+                   LTAKE_LAPPEND_fromList \\ strip_tac
+    \\ fs [])
+  \\ first_x_assum (qspec_then `SUC (LENGTH x)` mp_tac) \\ strip_tac
+  \\ fs [LPREFIX_fromList] \\ rfs []
+  \\ drule IS_PREFIX_LENGTH \\ strip_tac
+  \\ fs [REPLICATE_LIST_LENGTH]
+  \\ Cases_on `l` \\ Cases_on `LENGTH x` \\ fs [MULT_CLAUSES]
+QED
+
+Theorem printLoop_spec:
+  !s sv.
+    limited_parts names p /\ STRING_TYPE s sv ==>
+    app (p:'ffi ffi_proj) ^(fetch_v "printLoop" st) [sv]
+      (SIO []) (POSTd io. io = LREPEAT [put_str_event(s ^ strlit "\n")])
+Proof
+  xcf_div_rule IMP_app_POSTd_one_FFI_part_FLATTEN "printLoop" st
+  \\ MAP_EVERY qexists_tac
+    [`K emp`, `\i. if i = 0 then [] else [put_str_event(s ^ strlit "\n")]`, `K ($= sv)`,
+     `K State`, `update`]
+  \\ SIMP_TAC std_ss [LFLATTEN_LGENLIST_REPEAT,o_DEF,K_DEF,Once LGENLIST_NONE_UNFOLD,
+                      LFLATTEN_THM, CONJUNCT1 llistTheory.fromList_def]
+  \\ fs [GSYM SIO_def, REPLICATE_LIST_def]
+  \\ xsimpl
+  \\ xlet `POSTv v. &UNIT_TYPE () v *
+                    SIO [put_str_event(s ^ strlit "\n")]`
+  THEN1 (
+    xapp
+    \\ MAP_EVERY qexists_tac [`emp`, `s`, `[]`]
+    \\ xsimpl)
+  \\ xvar \\ xsimpl
+QED
+
+val sio_oracle = Define `
+  (sio_oracle:unit oracle) port st conf bytes =
+  if port = "put_char" then
+    Oracle_return st bytes
+  else Oracle_final FFI_failed
+`
+
+val encode_oracle_state_def = Define `
+  encode_oracle_state(st:unit) =
+      State`
+
+val decode_oracle_state_def = Define `
+  decode_oracle_state(st:ffi) = ()`
+
+Theorem decode_encode_oracle_state_11:
+  !ffi_st. decode_oracle_state(encode_oracle_state ffi_st) = ffi_st
+Proof
+  rw[encode_oracle_state_def,decode_oracle_state_def]
+QED
+
+val sio_proj1_def = Define `
+  sio_proj1 = (λffi.
+    FEMPTY |++ (mk_proj1 (encode_oracle_state,decode_oracle_state,
+                          [("put_char", sio_oracle "put_char")]) ffi))`;
+
+val sio_proj2 = Define `sio_proj2 =
+  [(["put_char"],update)]`
+
+Theorem limited_parts_proj:
+  limited_parts ["put_char"] (sio_proj1,sio_proj2)
+Proof
+  rw[limited_parts_def,sio_proj2]
+QED
+
+val sio_ffi_state_def = Define `sio_ffi_state =
+  <|oracle:=sio_oracle; ffi_state := (); io_events := []|>`;
+
+Theorem parts_ok_filter:
+  parts_ok sio_ffi_state (sio_proj1,sio_proj2)
+Proof
+  rw[cfStoreTheory.parts_ok_def,sio_proj1_def,sio_proj2,sio_ffi_state_def,
+     cfStoreTheory.ffi_has_index_in_def,mk_proj1_def,FLOOKUP_UPDATE,
+     FUPDATE_LIST_THM,FAPPLY_FUPDATE_THM,decode_encode_oracle_state_11,
+     sio_oracle,update_def]
+QED
+
+Theorem semantics_prog_thm:
+ semantics_prog ((^(get_state st)) with ffi:= sio_ffi_state) ^(get_env st)
+  (^maincall)
+  (Diverge(LREPEAT [put_str_event(strlit "yes\n")]))
+Proof
+  rpt strip_tac >>
+  `nsLookup ^(get_env st).v (Short "printLoop") = SOME printLoop_v`
+    by(unabbrev_all_tac >> EVAL_TAC) >>
+  assume_tac limited_parts_proj >>
+  FULL_SIMP_TAC bool_ss [GSYM names_def] >>
+  drule printLoop_spec >>
+  disch_then(qspec_then `strlit "yes"` mp_tac) >>
+  disch_then(qspec_then `Litv(StrLit "yes")` mp_tac) >>
+  simp[app_def,app_basic_def] >>
+  disch_then(mp_tac o CONV_RULE(RESORT_FORALL_CONV rev)) >>
+  qmatch_goalsub_abbrev_tac `semantics_prog st` >>
+  disch_then(qspec_then `st` mp_tac) >>
+  unabbrev_all_tac >>
+  simp[cfStoreTheory.st2heap_def,cfStoreTheory.store2heap_append,cfStoreTheory.ffi2heap_def,
+       miniBasisProg_st_def,parts_ok_filter,strcat_thm,implode_def] >>
+  qmatch_goalsub_abbrev_tac `FFI_split INSERT FFIset` >>
+  `FFIset = {FFI_part (encode_oracle_state ()) update
+                      ["put_char"] []}`
+    by(unabbrev_all_tac >> rw[FUN_EQ_THM,EQ_IMP_THM] >-
+        (pairarg_tac >> fs[sio_proj2] >> rveq >>
+         fs[] >>
+         fs[sio_proj1_def,mk_proj1_def] >>
+         fs[FLOOKUP_UPDATE,FUPDATE_LIST_THM,sio_ffi_state_def]) >>
+       Q.REFINE_EXISTS_TAC `(s,u,ns,ts)` >>
+       rw[sio_proj2,sio_ffi_state_def,sio_proj1_def,mk_proj1_def,
+          FLOOKUP_UPDATE,FUPDATE_LIST_THM]) >>
+  simp[] >> pop_assum kall_tac >> unabbrev_all_tac >>
+  qmatch_goalsub_abbrev_tac `junk ∪ {_;FFIpart}` >>
+  disch_then(qspecl_then [`FFI_split INSERT junk`,
+                          `{FFIpart}`]
+                         mp_tac) >>
+  impl_tac >-
+    (rw[SPLIT_def] >> unabbrev_all_tac >> simp[] >-
+       (rw[FUN_EQ_THM,EQ_IMP_THM] >> rw[]) >-
+       (simp[cfStoreTheory.FFI_part_NOT_IN_store2heap_aux,
+             cfStoreTheory.store2heap_def])
+    ) >>
+  impl_tac >- (simp[SIO_def,Abbr `FFIpart`,one_def,encode_oracle_state_def,names_def]) >>
+  strip_tac >>
+  Cases_on `r` >> fs[cond_def] >> rveq >>
+  fs[evaluate_to_heap_def,semanticsTheory.semantics_prog_def] >>
+  rpt strip_tac >-
+    (simp[semanticsTheory.evaluate_prog_with_clock_def,
+          terminationTheory.evaluate_decs_def,
+          astTheory.pat_bindings_def] >>
+     simp[terminationTheory.evaluate_def] >>
+     simp[semanticPrimitivesTheory.do_con_check_def,semanticPrimitivesTheory.build_conv_def] >>
+     rw[evaluateTheory.dec_clock_def] >>
+     fs[evaluate_ck_def] >>
+     first_x_assum(qspec_then `k - 1` strip_assume_tac) >>
+     fs[]) >>
+  fs[] >>
+  match_mp_tac(GEN_ALL lprefix_lub_subset) >>
+  goal_assum drule >> simp[] >> conj_tac >-
+    (rw[IMAGE_DEF,SUBSET_DEF] >>
+     qexists_tac `SUC ck` >>
+     simp[semanticsTheory.evaluate_prog_with_clock_def,
+          terminationTheory.evaluate_decs_def,
+          astTheory.pat_bindings_def
+         ] >>
+     simp[terminationTheory.evaluate_def] >>
+     simp[semanticPrimitivesTheory.do_con_check_def,semanticPrimitivesTheory.build_conv_def] >>
+     rw[evaluateTheory.dec_clock_def] >>
+     fs[evaluate_ck_def] >>
+     rpt(PURE_TOP_CASE_TAC >> rveq >> fs[])) >>
+  rw[PULL_EXISTS] >>
+  simp[LPREFIX_fromList_fromList] >>
+  simp[semanticsTheory.evaluate_prog_with_clock_def,
+       terminationTheory.evaluate_decs_def,
+       astTheory.pat_bindings_def
+      ] >>
+  simp[terminationTheory.evaluate_def] >>
+  simp[semanticPrimitivesTheory.do_con_check_def,semanticPrimitivesTheory.build_conv_def] >>
+  rw[evaluateTheory.dec_clock_def] >>
+  fs[evaluate_ck_def] >>
+  first_x_assum(qspec_then `k - 1` strip_assume_tac) >>
+  fs[] >-
+    (qexists_tac `ARB` >>
+     qmatch_goalsub_abbrev_tac `evaluate st` >>
+     Q.ISPEC_THEN `st` mp_tac
+       (CONJUNCT1 evaluatePropsTheory.evaluate_io_events_mono
+        |> SIMP_RULE std_ss [evaluatePropsTheory.io_events_mono_def]) >>
+     simp[Abbr `st`]) >>
+  qexists_tac `k - 1` >>
+  every_case_tac >> fs[]
+QED
+
+(* TODO: this proof is slow and also an abomination. We should really make proper
+   whole_prog_thm automation for Diverge.
+ *)
+Theorem yes_semantics_prog_Diverge:
+  let (s,env) = THE (prim_sem_env sio_ffi_state)
+  in semantics_prog s env yes_prog (Diverge (LREPEAT [put_str_event(strlit "yes\n")]))
+Proof
+  rw[] >>
+  mp_tac semantics_prog_thm >>
+  disch_then (mp_tac o CONV_RULE((RATOR_CONV o RATOR_CONV o RAND_CONV) EVAL)) >>
+  disch_then (mp_tac o CONV_RULE((RATOR_CONV o RATOR_CONV o RATOR_CONV o RAND_CONV) EVAL)) >>
+  CONV_TAC(RAND_CONV(RAND_CONV(RAND_CONV EVAL))) >>
+  fs[yes_prog_def,ml_progTheory.init_env_def] >>
+  (* TODO: can we avoid referring explicitly to these generated env defs in a cleaner way? *)
+  FULL_SIMP_TAC std_ss
+    (case st of ML_code (sts,envs,vs,_) => sts @ envs @ vs) >>
+  qabbrev_tac `maincall = ^maincall` >>
+  fs[semanticsTheory.semantics_prog_def,semanticsTheory.evaluate_prog_with_clock_def,
+     terminationTheory.evaluate_def,terminationTheory.evaluate_decs_def,
+     semanticPrimitivesTheory.check_dup_ctors_def,
+     astTheory.pat_bindings_def,
+     semanticPrimitivesTheory.combine_dec_result_def,
+     terminationTheory.pmatch_def,
+     semanticPrimitivesTheory.extend_dec_env_def,
+     semanticPrimitivesTheory.build_tdefs_def,
+     semanticPrimitivesTheory.build_constrs_def,
+     evaluatePropsTheory.evaluate_decs_cons,
+     ml_progTheory.write_def,
+     ml_progTheory.write_mod_def,
+     ml_progTheory.write_cons_def
+    ] >>
+  qmatch_goalsub_abbrev_tac `aa1  /\ aa2 ==> ab1 /\ ab2` >>
+  qsuff_tac `(aa1 = ab1) /\ (aa2 = ab2)` >-
+    (rpt(pop_assum kall_tac) >> metis_tac[]) >>
+  conj_tac >>
+  unabbrev_all_tac >>
+  CHANGED_TAC(rpt(AP_THM_TAC ORELSE AP_TERM_TAC)) >>
+  rw[FUN_EQ_THM,ELIM_UNCURRY] >>
+  qmatch_goalsub_abbrev_tac `evaluate_decs a1 a2` >>
+  qpat_abbrev_tac `aa1 = evaluate_decs a1 a2` >>
+  qmatch_goalsub_abbrev_tac `evaluate_decs a3 a4` >>
+  `a1 = a3`
+    by(unabbrev_all_tac >> simp[semanticPrimitivesTheory.state_component_equality]) >>
+  `a2 = a4`
+    by(unabbrev_all_tac >> EVAL_TAC) >>
+  simp[Abbr `aa1`] >>
+  Cases_on `evaluate_decs a3 a4 ^maincall` >> rw[] >>
+  rw[CaseEq"semanticPrimitives$result",CaseEq"prod"]
+QED
+
 val yes2_thm = compile_to_data (compilation_compset())
                                x64_backend_config_def
                                (REFL yes2)
@@ -1283,13 +1672,6 @@ Theorem backend_config_ok_yes:
   backend_config_ok yes_x64_conf
 Proof
  cheat
-QED
-
-Theorem yes_semantics_prog_Diverge:
-  let (s,env) = THE (prim_sem_env sio_ffi_state)
-  in semantics_prog s env yes_prog (Diverge (LREPEAT [put_char_event "yes\n"]))
-Proof
-  cheat
 QED
 
 Theorem yes_semantics_prog_not_Fail:
